Fix assumes/admits.

src/riot/RIoT.Core.fst
@@ -27,9 +27,60 @@ open RIoT.Impl
 
 module Ed25519 = Hacl.Ed25519
 
-#set-options "--z3rlimit 50 --fuel 0 --ifuel 0 --admit_smt_queries true"
+#set-options "--z3rlimit 50 --fuel 0 --ifuel 0 --using_facts_from '* -FStar.Tactics -FStar.Reflection'"
 
-#restart-solver
+noeq
+type deviceIDCSR_ingredients_t = {
+  deviceIDCSR_ku: key_usage_payload_t;
+  deviceIDCSR_version: datatype_of_asn1_type INTEGER;
+  deviceIDCSR_s_common:  x509_RDN_x520_attribute_string_t COMMON_NAME  IA5_STRING;
+  deviceIDCSR_s_org:     x509_RDN_x520_attribute_string_t ORGANIZATION IA5_STRING;
+  deviceIDCSR_s_country: x509_RDN_x520_attribute_string_t COUNTRY      PRINTABLE_STRING
+}
+
+noeq
+type aliasKeyCRT_ingredients_t = {
+  aliasKeyCrt_version: x509_version_t;
+  aliasKeyCrt_serialNumber: x509_serialNumber_t;
+  aliasKeyCrt_i_common:  x509_RDN_x520_attribute_string_t COMMON_NAME  IA5_STRING;
+  aliasKeyCrt_i_org:     x509_RDN_x520_attribute_string_t ORGANIZATION IA5_STRING;
+  aliasKeyCrt_i_country: x509_RDN_x520_attribute_string_t COUNTRY      PRINTABLE_STRING;
+  aliasKeyCrt_notBefore: datatype_of_asn1_type Generalized_Time;
+  aliasKeyCrt_notAfter : datatype_of_asn1_type Generalized_Time;
+  aliasKeyCrt_s_common:  x509_RDN_x520_attribute_string_t COMMON_NAME  IA5_STRING;
+  aliasKeyCrt_s_org:     x509_RDN_x520_attribute_string_t ORGANIZATION IA5_STRING;
+  aliasKeyCrt_s_country: x509_RDN_x520_attribute_string_t COUNTRY      PRINTABLE_STRING;
+  aliasKeyCrt_ku: key_usage_payload_t;
+  aliasKeyCrt_riot_version: datatype_of_asn1_type INTEGER;
+}
+
+let deviceIDCRI_pre (x:deviceIDCSR_ingredients_t) =
+  valid_deviceIDCRI_ingredients
+    x.deviceIDCSR_version x.deviceIDCSR_s_common x.deviceIDCSR_s_org x.deviceIDCSR_s_country x.deviceIDCSR_ku
+
+[@@ "opaque_to_smt"]
+unfold noextract
+let coerce_asn1_tlv_int32_of_type_to_asn1_int32 (x:asn1_TLV_int32_of_type SEQUENCE)
+  : asn1_int32 = x
+
+let deviceIDCSR_pre (x:deviceIDCSR_ingredients_t{deviceIDCRI_pre x}) (deviceIDCSR_len:UInt32.t) =
+  let l = coerce_asn1_tlv_int32_of_type_to_asn1_int32
+    (len_of_deviceIDCRI
+      x.deviceIDCSR_version x.deviceIDCSR_s_common x.deviceIDCSR_s_org
+      x.deviceIDCSR_s_country x.deviceIDCSR_ku) in
+  
+  valid_deviceIDCSR_ingredients l /\
+  eq2 #nat (v deviceIDCSR_len) (length_of_deviceIDCSR l)
+
+let aliasKeyCRT_pre (x:aliasKeyCRT_ingredients_t) (aliasKeyCRT_len:UInt32.t) =
+  let l = coerce_asn1_tlv_int32_of_type_to_asn1_int32
+    (len_of_aliasKeyTBS
+      x.aliasKeyCrt_serialNumber x.aliasKeyCrt_i_common x.aliasKeyCrt_i_org x.aliasKeyCrt_i_country
+      x.aliasKeyCrt_s_common x.aliasKeyCrt_s_org x.aliasKeyCrt_s_country x.aliasKeyCrt_ku
+      x.aliasKeyCrt_riot_version) in
+  valid_aliasKeyCRT_ingredients l /\
+  eq2 #nat (v aliasKeyCRT_len) (length_of_aliasKeyCRT l)
+
 let riot_pre
   (h: HS.mem)
 (* Common Inputs *)
@@ -40,9 +91,9 @@ let riot_pre
   (aliasKey_label_len: size_t)
   (aliasKey_label: B.lbuffer byte_sec (v aliasKey_label_len))
 (* DeviceID CSR Inputs*)
-  (deviceIDCSR_ingredients: deviceIDCSR_ingredients_t)
+  (deviceIDCSR_ingredients:deviceIDCSR_ingredients_t)
 (* AliasKey Crt Inputs*)
-  (aliasKeyCRT_ingredients: aliasKeyCRT_ingredients_t)
+  (aliasKeyCRT_ingredients:aliasKeyCRT_ingredients_t)
 (* Common Outputs *)
   (aliasKey_pub: B.lbuffer byte_pub 32)
   (aliasKey_priv: B.lbuffer uint8 32)
@@ -72,268 +123,121 @@ let riot_pre
    (* Pre: labels have enough length for HKDF *)
    valid_hkdf_lbl_len deviceID_label_len /\
    valid_hkdf_lbl_len aliasKey_label_len /\
-   (* Pre: DeviceIDCSR will have a valid length *)
-   valid_deviceIDCSR_ingredients
-     (len_of_deviceIDCRI
-       deviceIDCSR_ingredients.deviceIDCSR_version
-       deviceIDCSR_ingredients.deviceIDCSR_s_common
-       deviceIDCSR_ingredients.deviceIDCSR_s_org
-       deviceIDCSR_ingredients.deviceIDCSR_s_country) /\
-   (* Pre: `deviceIDCSR_buf` has exact size to write DeviceIDCSR *)
-   v deviceIDCSR_len == length_of_deviceIDCSR
-                          (len_of_deviceIDCRI
-                            deviceIDCSR_ingredients.deviceIDCSR_version
-                            deviceIDCSR_ingredients.deviceIDCSR_s_common
-                            deviceIDCSR_ingredients.deviceIDCSR_s_org
-                            deviceIDCSR_ingredients.deviceIDCSR_s_country) /\
-   (* Pre: AliasKeyTBS will have a valid length *)
-   valid_aliasKeyCRT_ingredients
-     (len_of_aliasKeyTBS
-       aliasKeyCRT_ingredients.aliasKeyCrt_serialNumber
-       aliasKeyCRT_ingredients.aliasKeyCrt_i_common
-       aliasKeyCRT_ingredients.aliasKeyCrt_i_org
-       aliasKeyCRT_ingredients.aliasKeyCrt_i_country
-       aliasKeyCRT_ingredients.aliasKeyCrt_s_common
-       aliasKeyCRT_ingredients.aliasKeyCrt_s_org
-       aliasKeyCRT_ingredients.aliasKeyCrt_s_country
-       aliasKeyCRT_ingredients.aliasKeyCrt_riot_version) /\
-   (* Pre: `aliasKeyCRT_buf` has exact size to write AliasKeyCRT *)
-   v aliasKeyCRT_len == length_of_aliasKeyCRT
-                          (len_of_aliasKeyTBS
-                             aliasKeyCRT_ingredients.aliasKeyCrt_serialNumber
-                             aliasKeyCRT_ingredients.aliasKeyCrt_i_common
-                             aliasKeyCRT_ingredients.aliasKeyCrt_i_org
-                             aliasKeyCRT_ingredients.aliasKeyCrt_i_country
-                             aliasKeyCRT_ingredients.aliasKeyCrt_s_common
-                             aliasKeyCRT_ingredients.aliasKeyCrt_s_org
-                             aliasKeyCRT_ingredients.aliasKeyCrt_s_country
-                             aliasKeyCRT_ingredients.aliasKeyCrt_riot_version)
 
-let riot_post_modifies
-  (h0: HS.mem) (r: unit) (h1: HS.mem)
-(* Common Inputs *)
-  (cdi : B.lbuffer byte_sec 32)
-  (fwid: B.lbuffer byte_sec 32)
-  (deviceID_label_len: size_t)
-  (deviceID_label: B.lbuffer byte_sec (v deviceID_label_len))
-  (aliasKey_label_len: size_t)
+   deviceIDCRI_pre deviceIDCSR_ingredients /\
+   deviceIDCSR_pre deviceIDCSR_ingredients deviceIDCSR_len /\
+   aliasKeyCRT_pre aliasKeyCRT_ingredients aliasKeyCRT_len
+
+let aliasKey_post
+  (cdi : B.lbuffer byte_sec 32) (fwid: B.lbuffer byte_sec 32)
+  (aliasKey_label_len:UInt32.t{valid_hkdf_lbl_len aliasKey_label_len})
   (aliasKey_label: B.lbuffer byte_sec (v aliasKey_label_len))
-(* DeviceID CSR Inputs*)
-  (deviceIDCSR_ingredients: deviceIDCSR_ingredients_t)
-(* AliasKey Crt Inputs*)
-  (aliasKeyCRT_ingredients: aliasKeyCRT_ingredients_t)
-(* Common Outputs *)
   (aliasKey_pub: B.lbuffer byte_pub 32)
   (aliasKey_priv: B.lbuffer uint8 32)
-(* DeviceID CSR Outputs *)
-  (deviceIDCSR_len: size_t)
-  (deviceIDCSR_buf: B.lbuffer byte_pub (v deviceIDCSR_len))
-(* AliasKey Crt Outputs *)
-  (aliasKeyCRT_len: size_t)
-  (aliasKeyCRT_buf: B.lbuffer byte_pub (v aliasKeyCRT_len)
-                    { riot_pre
-                        (h0)
-                        (cdi)
-                        (fwid)
-                        (deviceID_label_len) (deviceID_label)
-                        (aliasKey_label_len) (aliasKey_label)
-                        (deviceIDCSR_ingredients)
-                        (aliasKeyCRT_ingredients)
-                        (aliasKey_pub)
-                        (aliasKey_priv)
-                        (deviceIDCSR_len) (deviceIDCSR_buf)
-                        (aliasKeyCRT_len) (aliasKeyCRT_buf) })
-: Type0
-=   (* Post: Modifies *)
-     B.(modifies (loc_buffer deviceIDCSR_buf `loc_union`
-                  loc_buffer aliasKeyCRT_buf `loc_union`
-                  loc_buffer aliasKey_pub    `loc_union`
-                  loc_buffer aliasKey_priv ) h0 h1)
+  (h0 h1:HS.mem)
+ = ((B.as_seq h1 aliasKey_pub  <: lbytes_pub 32),
+    (B.as_seq h1 aliasKey_priv <: lbytes_sec 32)) == derive_AliasKey_spec
+                                                       (B.as_seq h0 cdi)
+                                                       (B.as_seq h0 fwid)
+                                                       aliasKey_label_len
+                                                       (B.as_seq h0 aliasKey_label)
 
-let riot_post_aliasKey
-  (h0: HS.mem) (r: unit) (h1: HS.mem)
-(* Common Inputs *)
-  (cdi : B.lbuffer byte_sec 32)
-  (fwid: B.lbuffer byte_sec 32)
-  (deviceID_label_len: size_t)
-  (deviceID_label: B.lbuffer byte_sec (v deviceID_label_len))
-  (aliasKey_label_len: size_t)
-  (aliasKey_label: B.lbuffer byte_sec (v aliasKey_label_len))
-(* DeviceID CSR Inputs*)
-  (deviceIDCSR_ingredients: deviceIDCSR_ingredients_t)
-(* AliasKey Crt Inputs*)
-  (aliasKeyCRT_ingredients: aliasKeyCRT_ingredients_t)
-(* Common Outputs *)
-  (aliasKey_pub: B.lbuffer byte_pub 32)
-  (aliasKey_priv: B.lbuffer uint8 32)
-(* DeviceID CSR Outputs *)
-  (deviceIDCSR_len: size_t)
-  (deviceIDCSR_buf: B.lbuffer byte_pub (v deviceIDCSR_len))
-(* AliasKey Crt Outputs *)
-  (aliasKeyCRT_len: size_t)
-  (aliasKeyCRT_buf: B.lbuffer byte_pub (v aliasKeyCRT_len)
-                    { riot_pre
-                        (h0)
-                        (cdi)
-                        (fwid)
-                        (deviceID_label_len) (deviceID_label)
-                        (aliasKey_label_len) (aliasKey_label)
-                        (deviceIDCSR_ingredients)
-                        (aliasKeyCRT_ingredients)
-                        (aliasKey_pub)
-                        (aliasKey_priv)
-                        (deviceIDCSR_len) (deviceIDCSR_buf)
-                        (aliasKeyCRT_len) (aliasKeyCRT_buf) })
-: Type0
-=   (* Post: AliasKey *)
-    ((B.as_seq h1 aliasKey_pub  <: lbytes_pub 32),
-     (B.as_seq h1 aliasKey_priv <: lbytes_sec 32)) == derive_AliasKey_spec
-                                                        (B.as_seq h0 cdi)
-                                                        (B.as_seq h0 fwid)
-                                                        aliasKey_label_len
-                                                        (B.as_seq h0 aliasKey_label)
+#push-options "--z3rlimit 100"
+let deviceIDCSR_post
+  (cdi:B.lbuffer byte_sec 32)
+  (deviceID_label_len:UInt32.t{valid_hkdf_lbl_len deviceID_label_len})
+  (deviceID_label:B.lbuffer byte_sec (v deviceID_label_len))
+  (deviceIDCSR_ingredients:deviceIDCSR_ingredients_t)
+  (deviceIDCSR_len:UInt32.t{
+    deviceIDCRI_pre deviceIDCSR_ingredients /\
+    deviceIDCSR_pre deviceIDCSR_ingredients deviceIDCSR_len})
+  (deviceIDCSR_buf:B.lbuffer byte_pub (v deviceIDCSR_len))
+  (h0 h1:HS.mem)
+  = let deviceID_pub_seq, deviceID_priv_seq = derive_DeviceID_spec
+                                                (B.as_seq h0 cdi)
+                                                (deviceID_label_len)
+                                                (B.as_seq h0 deviceID_label) in
+    let deviceIDCRI: deviceIDCRI_t = create_deviceIDCRI_spec
+      deviceIDCSR_ingredients.deviceIDCSR_version deviceIDCSR_ingredients.deviceIDCSR_s_common
+      deviceIDCSR_ingredients.deviceIDCSR_s_org deviceIDCSR_ingredients.deviceIDCSR_s_country
+      deviceIDCSR_ingredients.deviceIDCSR_ku deviceID_pub_seq in
 
-let riot_post_aliasKeyCrt
-  (h0: HS.mem) (r: unit) (h1: HS.mem)
-(* Common Inputs *)
-  (cdi : B.lbuffer byte_sec 32)
+    let deviceIDCRI_seq = serialize_deviceIDCRI `serialize` deviceIDCRI in
+    
+    let deviceIDCRI_len = coerce_asn1_tlv_int32_of_type_to_asn1_int32
+      (len_of_deviceIDCRI
+        deviceIDCSR_ingredients.deviceIDCSR_version deviceIDCSR_ingredients.deviceIDCSR_s_common
+        deviceIDCSR_ingredients.deviceIDCSR_s_org deviceIDCSR_ingredients.deviceIDCSR_s_country
+        deviceIDCSR_ingredients.deviceIDCSR_ku) in
+      
+    let (* Prf *) _ = lemma_serialize_deviceIDCRI_size_exact deviceIDCRI in  //AR: TODO: This takes long time
+    let deviceIDCSR: deviceIDCSR_t deviceIDCRI_len = sign_and_finalize_deviceIDCSR_spec
+                                                                (deviceID_priv_seq)
+                                                                (deviceIDCRI_len)
+                                                                (deviceIDCRI_seq) in
+    B.as_seq h1 deviceIDCSR_buf == serialize_deviceIDCSR deviceIDCRI_len `serialize` deviceIDCSR
+#pop-options
+
+unfold noextract
+let coerce_asn1_int32_to_size_t (x:asn1_int32) : size_t = x
+
+#push-options "--z3rlimit 100"
+let aliasKeyCRT_post
+  (cdi:B.lbuffer byte_sec 32)
   (fwid: B.lbuffer byte_sec 32)
-  (deviceID_label_len: size_t)
-  (deviceID_label: B.lbuffer byte_sec (v deviceID_label_len))
-  (aliasKey_label_len: size_t)
-  (aliasKey_label: B.lbuffer byte_sec (v aliasKey_label_len))
-(* DeviceID CSR Inputs*)
-  (deviceIDCSR_ingredients: deviceIDCSR_ingredients_t)
-(* AliasKey Crt Inputs*)
-  (aliasKeyCRT_ingredients: aliasKeyCRT_ingredients_t)
-(* Common Outputs *)
+  (deviceID_label_len:UInt32.t{valid_hkdf_lbl_len deviceID_label_len})
+  (deviceID_label:B.lbuffer byte_sec (v deviceID_label_len))
+  (aliasKeyCRT_ingredients:aliasKeyCRT_ingredients_t)
+  (aliasKeyCRT_len:UInt32.t{
+    aliasKeyCRT_pre aliasKeyCRT_ingredients aliasKeyCRT_len})
+  (aliasKeyCRT_buf: B.lbuffer byte_pub (v aliasKeyCRT_len))
   (aliasKey_pub: B.lbuffer byte_pub 32)
-  (aliasKey_priv: B.lbuffer uint8 32)
-(* DeviceID CSR Outputs *)
-  (deviceIDCSR_len: size_t)
-  (deviceIDCSR_buf: B.lbuffer byte_pub (v deviceIDCSR_len))
-(* AliasKey Crt Outputs *)
-  (aliasKeyCRT_len: size_t)
-  (aliasKeyCRT_buf: B.lbuffer byte_pub (v aliasKeyCRT_len)
-                    { riot_pre
-                        (h0)
-                        (cdi)
-                        (fwid)
-                        (deviceID_label_len) (deviceID_label)
-                        (aliasKey_label_len) (aliasKey_label)
-                        (deviceIDCSR_ingredients)
-                        (aliasKeyCRT_ingredients)
-                        (aliasKey_pub)
-                        (aliasKey_priv)
-                        (deviceIDCSR_len) (deviceIDCSR_buf)
-                        (aliasKeyCRT_len) (aliasKeyCRT_buf) })
-: Type0
-=   (* Post: AliasKeyCRT *)
-    (let deviceID_pub_seq, deviceID_priv_seq = derive_DeviceID_spec
+  (h0 h1:HS.mem)
+  = let deviceID_pub_seq, deviceID_priv_seq = derive_DeviceID_spec
                                                  (B.as_seq h0 cdi)
                                                  (deviceID_label_len)
                                                  (B.as_seq h0 deviceID_label) in
-     let aliasKeyCrt_keyID_seq: lbytes_pub 20 =
-       derive_authKeyID_from_cdi_spec (B.as_seq h0 cdi) (deviceID_label_len) (B.as_seq h0 deviceID_label) in
-     let aliasKeyCrt_keyID = sha1_digest_to_octet_string_spec aliasKeyCrt_keyID_seq in
-     let aliasKeyTBS = create_aliasKeyTBS_spec
-                                        (aliasKeyCRT_ingredients.aliasKeyCrt_version)
-                                        (aliasKeyCRT_ingredients.aliasKeyCrt_serialNumber)
-                                        (aliasKeyCRT_ingredients.aliasKeyCrt_i_common)
-                                        (aliasKeyCRT_ingredients.aliasKeyCrt_i_org)
-                                        (aliasKeyCRT_ingredients.aliasKeyCrt_i_country)
-                                        (aliasKeyCRT_ingredients.aliasKeyCrt_notBefore)
-                                        (aliasKeyCRT_ingredients.aliasKeyCrt_notAfter)
-                                        (aliasKeyCRT_ingredients.aliasKeyCrt_s_common)
-                                        (aliasKeyCRT_ingredients.aliasKeyCrt_s_org)
-                                        (aliasKeyCRT_ingredients.aliasKeyCrt_s_country)
-                                        (aliasKeyCRT_ingredients.aliasKeyCrt_ku)
-                                        (aliasKeyCrt_keyID)
-                                        (aliasKeyCRT_ingredients.aliasKeyCrt_riot_version)
-                                        (B.as_seq h0 fwid)
-                                        (deviceID_pub_seq)
-                                        (B.as_seq h1 aliasKey_pub)
-                                        in
+    let aliasKeyCrt_keyID_seq: lbytes_pub 20 =
+     derive_authKeyID_from_cdi_spec (B.as_seq h0 cdi) (deviceID_label_len) (B.as_seq h0 deviceID_label) in
+    let aliasKeyTBS = create_aliasKeyTBS_spec
+      aliasKeyCRT_ingredients.aliasKeyCrt_version
+      aliasKeyCRT_ingredients.aliasKeyCrt_serialNumber
+      aliasKeyCRT_ingredients.aliasKeyCrt_i_common
+      aliasKeyCRT_ingredients.aliasKeyCrt_i_org
+      aliasKeyCRT_ingredients.aliasKeyCrt_i_country
+      aliasKeyCRT_ingredients.aliasKeyCrt_notBefore
+      aliasKeyCRT_ingredients.aliasKeyCrt_notAfter
+      aliasKeyCRT_ingredients.aliasKeyCrt_s_common
+      aliasKeyCRT_ingredients.aliasKeyCrt_s_org
+      aliasKeyCRT_ingredients.aliasKeyCrt_s_country
+      aliasKeyCRT_ingredients.aliasKeyCrt_ku
+      aliasKeyCrt_keyID_seq
+      aliasKeyCRT_ingredients.aliasKeyCrt_riot_version
+      (B.as_seq h0 fwid)
+      deviceID_pub_seq
+      (B.as_seq h1 aliasKey_pub) in
      let aliasKeyTBS_seq = serialize_aliasKeyTBS `serialize` aliasKeyTBS in
-     let aliasKeyTBS_len = len_of_aliasKeyTBS
-                             aliasKeyCRT_ingredients.aliasKeyCrt_serialNumber
-                             aliasKeyCRT_ingredients.aliasKeyCrt_i_common
-                             aliasKeyCRT_ingredients.aliasKeyCrt_i_org
-                             aliasKeyCRT_ingredients.aliasKeyCrt_i_country
-                             aliasKeyCRT_ingredients.aliasKeyCrt_s_common
-                             aliasKeyCRT_ingredients.aliasKeyCrt_s_org
-                             aliasKeyCRT_ingredients.aliasKeyCrt_s_country
-                             aliasKeyCRT_ingredients.aliasKeyCrt_riot_version in
+     let aliasKeyTBS_len = coerce_asn1_tlv_int32_of_type_to_asn1_int32
+       (len_of_aliasKeyTBS
+         aliasKeyCRT_ingredients.aliasKeyCrt_serialNumber
+         aliasKeyCRT_ingredients.aliasKeyCrt_i_common
+         aliasKeyCRT_ingredients.aliasKeyCrt_i_org
+         aliasKeyCRT_ingredients.aliasKeyCrt_i_country
+         aliasKeyCRT_ingredients.aliasKeyCrt_s_common
+         aliasKeyCRT_ingredients.aliasKeyCrt_s_org
+         aliasKeyCRT_ingredients.aliasKeyCrt_s_country
+         aliasKeyCRT_ingredients.aliasKeyCrt_ku
+         aliasKeyCRT_ingredients.aliasKeyCrt_riot_version) in
      let (* Prf *) _ = lemma_serialize_aliasKeyTBS_size_exact aliasKeyTBS in
+     assume (Seq.length aliasKeyTBS_seq == v aliasKeyTBS_len); //TODO: help Z3 prove it
      let aliasKeyCRT: aliasKeyCRT_t aliasKeyTBS_len = sign_and_finalize_aliasKeyCRT_spec
                                                                 (deviceID_priv_seq)
                                                                 (aliasKeyTBS_len)
                                                                 (aliasKeyTBS_seq) in
-     B.as_seq h1 aliasKeyCRT_buf == serialize_aliasKeyCRT aliasKeyTBS_len `serialize` aliasKeyCRT)
+     B.as_seq h1 aliasKeyCRT_buf == serialize_aliasKeyCRT aliasKeyTBS_len `serialize` aliasKeyCRT
 
-let riot_post_deviceIDCSR
-  (h0: HS.mem) (r: unit) (h1: HS.mem)
-(* Common Inputs *)
-  (cdi : B.lbuffer byte_sec 32)
-  (fwid: B.lbuffer byte_sec 32)
-  (deviceID_label_len: size_t)
-  (deviceID_label: B.lbuffer byte_sec (v deviceID_label_len))
-  (aliasKey_label_len: size_t)
-  (aliasKey_label: B.lbuffer byte_sec (v aliasKey_label_len))
-(* DeviceID CSR Inputs*)
-  (deviceIDCSR_ingredients: deviceIDCSR_ingredients_t)
-(* AliasKey Crt Inputs*)
-  (aliasKeyCRT_ingredients: aliasKeyCRT_ingredients_t)
-(* Common Outputs *)
-  (aliasKey_pub: B.lbuffer byte_pub 32)
-  (aliasKey_priv: B.lbuffer uint8 32)
-(* DeviceID CSR Outputs *)
-  (deviceIDCSR_len: size_t)
-  (deviceIDCSR_buf: B.lbuffer byte_pub (v deviceIDCSR_len))
-(* AliasKey Crt Outputs *)
-  (aliasKeyCRT_len: size_t)
-  (aliasKeyCRT_buf: B.lbuffer byte_pub (v aliasKeyCRT_len)
-                    { riot_pre
-                        (h0)
-                        (cdi)
-                        (fwid)
-                        (deviceID_label_len) (deviceID_label)
-                        (aliasKey_label_len) (aliasKey_label)
-                        (deviceIDCSR_ingredients)
-                        (aliasKeyCRT_ingredients)
-                        (aliasKey_pub)
-                        (aliasKey_priv)
-                        (deviceIDCSR_len) (deviceIDCSR_buf)
-                        (aliasKeyCRT_len) (aliasKeyCRT_buf) })
-: Type0
-=   (* Post: AliasKeyCRT *)
-    (let deviceID_pub_seq, deviceID_priv_seq = derive_DeviceID_spec
-                                                 (B.as_seq h0 cdi)
-                                                 (deviceID_label_len)
-                                                 (B.as_seq h0 deviceID_label) in
-     let deviceIDCRI: deviceIDCRI_t = create_deviceIDCRI_spec
-                                                                         (deviceIDCSR_ingredients.deviceIDCSR_version)
-                                                                         (deviceIDCSR_ingredients.deviceIDCSR_s_common)
-                                                                         (deviceIDCSR_ingredients.deviceIDCSR_s_org)
-                                                                         (deviceIDCSR_ingredients.deviceIDCSR_s_country)
-                                                                         (deviceIDCSR_ingredients.deviceIDCSR_ku)
-                                                                         (deviceID_pub_seq)
-                                                                         in
-     let deviceIDCRI_seq = serialize_deviceIDCRI `serialize` deviceIDCRI in
-     let deviceIDCRI_len = len_of_deviceIDCRI
-                             deviceIDCSR_ingredients.deviceIDCSR_version
-                             deviceIDCSR_ingredients.deviceIDCSR_s_common
-                             deviceIDCSR_ingredients.deviceIDCSR_s_org
-                             deviceIDCSR_ingredients.deviceIDCSR_s_country in
-     let (* Prf *) _ = lemma_serialize_deviceIDCRI_size_exact deviceIDCRI in
-     let deviceIDCSR: deviceIDCSR_t deviceIDCRI_len = sign_and_finalize_deviceIDCSR_spec
-                                                                (deviceID_priv_seq)
-                                                                (deviceIDCRI_len)
-                                                                (deviceIDCRI_seq) in
-     B.as_seq h1 deviceIDCSR_buf == serialize_deviceIDCSR deviceIDCRI_len `serialize` deviceIDCSR)
 
 let riot_post
-  (h0: HS.mem) (r: unit) (h1: HS.mem)
 (* Common Inputs *)
   (cdi : B.lbuffer byte_sec 32)
   (fwid: B.lbuffer byte_sec 32)
@@ -342,73 +246,39 @@ let riot_post
   (aliasKey_label_len: size_t)
   (aliasKey_label: B.lbuffer byte_sec (v aliasKey_label_len))
 (* DeviceID CSR Inputs*)
-  (deviceIDCSR_ingredients: deviceIDCSR_ingredients_t)
+  (deviceIDCSR_ingredients:deviceIDCSR_ingredients_t)
 (* AliasKey Crt Inputs*)
-  (aliasKeyCRT_ingredients: aliasKeyCRT_ingredients_t)
+  (aliasKeyCRT_ingredients:aliasKeyCRT_ingredients_t)
 (* Common Outputs *)
   (aliasKey_pub: B.lbuffer byte_pub 32)
   (aliasKey_priv: B.lbuffer uint8 32)
 (* DeviceID CSR Outputs *)
-  (deviceIDCSR_len: size_t)
+  (deviceIDCSR_len: UInt32.t)
   (deviceIDCSR_buf: B.lbuffer byte_pub (v deviceIDCSR_len))
 (* AliasKey Crt Outputs *)
-  (aliasKeyCRT_len: size_t)
-  (aliasKeyCRT_buf: B.lbuffer byte_pub (v aliasKeyCRT_len)
-                    { riot_pre
-                        (h0)
-                        (cdi)
-                        (fwid)
-                        (deviceID_label_len) (deviceID_label)
-                        (aliasKey_label_len) (aliasKey_label)
-                        (deviceIDCSR_ingredients)
-                        (aliasKeyCRT_ingredients)
-                        (aliasKey_pub)
-                        (aliasKey_priv)
-                        (deviceIDCSR_len) (deviceIDCSR_buf)
-                        (aliasKeyCRT_len) (aliasKeyCRT_buf) })
-: Type0
-=  riot_post_modifies
-                        (h0) () (h1)
-                        (cdi) (fwid)
-                        (deviceID_label_len) (deviceID_label)
-                        (aliasKey_label_len) (aliasKey_label)
-                        (deviceIDCSR_ingredients)
-                        (aliasKeyCRT_ingredients)
-                        (aliasKey_pub) (aliasKey_priv)
-                        (deviceIDCSR_len) (deviceIDCSR_buf)
-                        (aliasKeyCRT_len) (aliasKeyCRT_buf) /\
-   riot_post_aliasKey
-                        (h0) () (h1)
-                        (cdi) (fwid)
-                        (deviceID_label_len) (deviceID_label)
-                        (aliasKey_label_len) (aliasKey_label)
-                        (deviceIDCSR_ingredients)
-                        (aliasKeyCRT_ingredients)
-                        (aliasKey_pub) (aliasKey_priv)
-                        (deviceIDCSR_len) (deviceIDCSR_buf)
-                        (aliasKeyCRT_len) (aliasKeyCRT_buf) /\
-   riot_post_aliasKeyCrt
-                        (h0) () (h1)
-                        (cdi) (fwid)
-                        (deviceID_label_len) (deviceID_label)
-                        (aliasKey_label_len) (aliasKey_label)
-                        (deviceIDCSR_ingredients)
-                        (aliasKeyCRT_ingredients)
-                        (aliasKey_pub) (aliasKey_priv)
-                        (deviceIDCSR_len) (deviceIDCSR_buf)
-                        (aliasKeyCRT_len) (aliasKeyCRT_buf) /\
-   riot_post_deviceIDCSR
-                        (h0) () (h1)
-                        (cdi) (fwid)
-                        (deviceID_label_len) (deviceID_label)
-                        (aliasKey_label_len) (aliasKey_label)
-                        (deviceIDCSR_ingredients)
-                        (aliasKeyCRT_ingredients)
-                        (aliasKey_pub) (aliasKey_priv)
-                        (deviceIDCSR_len) (deviceIDCSR_buf)
-                        (aliasKeyCRT_len) (aliasKeyCRT_buf)
+  (aliasKeyCRT_len: UInt32.t)
+  (aliasKeyCRT_buf: B.lbuffer byte_pub (v aliasKeyCRT_len))
+  (h0:HS.mem{
+    riot_pre h0 cdi fwid deviceID_label_len deviceID_label
+    aliasKey_label_len aliasKey_label deviceIDCSR_ingredients
+    aliasKeyCRT_ingredients aliasKey_pub aliasKey_priv
+    deviceIDCSR_len deviceIDCSR_buf
+    aliasKeyCRT_len aliasKeyCRT_buf})
+  (h1:HS.mem) 
+  : Type0
+  = B.(modifies (loc_buffer deviceIDCSR_buf `loc_union`
+                 loc_buffer aliasKeyCRT_buf `loc_union`
+                 loc_buffer aliasKey_pub    `loc_union`
+                 loc_buffer aliasKey_priv ) h0 h1) /\
 
-#restart-solver
+    aliasKey_post cdi fwid aliasKey_label_len aliasKey_label aliasKey_pub aliasKey_priv h0 h1 /\
+    
+    deviceIDCSR_post cdi deviceID_label_len deviceID_label
+      deviceIDCSR_ingredients deviceIDCSR_len deviceIDCSR_buf h0 h1 /\
+    
+    aliasKeyCRT_post cdi fwid deviceID_label_len deviceID_label
+      aliasKeyCRT_ingredients aliasKeyCRT_len aliasKeyCRT_buf aliasKey_pub h0 h1
+
 let riot
 (* Common Inputs *)
   (cdi : B.lbuffer byte_sec 32)
@@ -418,9 +288,24 @@ let riot
   (aliasKey_label_len: size_t)
   (aliasKey_label: B.lbuffer byte_sec (v aliasKey_label_len))
 (* DeviceID CSR Inputs*)
-  (deviceIDCSR_ingredients: deviceIDCSR_ingredients_t)
+  (deviceIDCSR_ku: key_usage_payload_t)
+  (deviceIDCSR_version: datatype_of_asn1_type INTEGER)
+  (deviceIDCSR_s_common:  x509_RDN_x520_attribute_string_t COMMON_NAME  IA5_STRING)
+  (deviceIDCSR_s_org:     x509_RDN_x520_attribute_string_t ORGANIZATION IA5_STRING)
+  (deviceIDCSR_s_country: x509_RDN_x520_attribute_string_t COUNTRY      PRINTABLE_STRING)
 (* AliasKey Crt Inputs*)
-  (aliasKeyCRT_ingredients: aliasKeyCRT_ingredients_t)
+  (aliasKeyCrt_version: x509_version_t)
+  (aliasKeyCrt_serialNumber: x509_serialNumber_t)
+  (aliasKeyCrt_i_common:  x509_RDN_x520_attribute_string_t COMMON_NAME  IA5_STRING)
+  (aliasKeyCrt_i_org:     x509_RDN_x520_attribute_string_t ORGANIZATION IA5_STRING)
+  (aliasKeyCrt_i_country: x509_RDN_x520_attribute_string_t COUNTRY      PRINTABLE_STRING)
+  (aliasKeyCrt_notBefore: datatype_of_asn1_type Generalized_Time)
+  (aliasKeyCrt_notAfter : datatype_of_asn1_type Generalized_Time)
+  (aliasKeyCrt_s_common:  x509_RDN_x520_attribute_string_t COMMON_NAME  IA5_STRING)
+  (aliasKeyCrt_s_org:     x509_RDN_x520_attribute_string_t ORGANIZATION IA5_STRING)
+  (aliasKeyCrt_s_country: x509_RDN_x520_attribute_string_t COUNTRY      PRINTABLE_STRING)
+  (aliasKeyCrt_ku: key_usage_payload_t)
+  (riot_version: datatype_of_asn1_type INTEGER)
 (* Common Outputs *)
   (aliasKey_pub: B.lbuffer byte_pub 32)
   (aliasKey_priv: B.lbuffer uint8 32)
@@ -432,23 +317,44 @@ let riot
   (aliasKeyCRT_buf: B.lbuffer byte_pub (v aliasKeyCRT_len))
 : HST.Stack unit
   (requires fun h -> riot_pre
-                        (h) (cdi) (fwid)
+                        (h)
+                        (cdi)
+                        (fwid)
                         (deviceID_label_len) (deviceID_label)
                         (aliasKey_label_len) (aliasKey_label)
-                        (deviceIDCSR_ingredients)
-                        (aliasKeyCRT_ingredients)
-                        (aliasKey_pub) (aliasKey_priv)
+                        (deviceIDCSR_ku)
+                        (deviceIDCSR_version)
+                        (deviceIDCSR_s_common) (deviceIDCSR_s_org) (deviceIDCSR_s_country)
+                        (aliasKeyCrt_version)
+                        (aliasKeyCrt_serialNumber)
+                        (aliasKeyCrt_i_common) (aliasKeyCrt_i_org) (aliasKeyCrt_i_country)
+                        (aliasKeyCrt_notBefore) (aliasKeyCrt_notAfter)
+                        (aliasKeyCrt_s_common) (aliasKeyCrt_s_org) (aliasKeyCrt_s_country)
+                        (aliasKeyCrt_ku)
+                        (riot_version)
+                        (aliasKey_pub)
+                        (aliasKey_priv)
                         (deviceIDCSR_len) (deviceIDCSR_buf)
                         (aliasKeyCRT_len) (aliasKeyCRT_buf)
    )
    (ensures fun h0 _ h1 -> riot_post
                         (h0) () (h1)
-                        (cdi) (fwid)
+                        (cdi)
+                        (fwid)
                         (deviceID_label_len) (deviceID_label)
                         (aliasKey_label_len) (aliasKey_label)
-                        (deviceIDCSR_ingredients)
-                        (aliasKeyCRT_ingredients)
-                        (aliasKey_pub) (aliasKey_priv)
+                        (deviceIDCSR_ku)
+                        (deviceIDCSR_version)
+                        (deviceIDCSR_s_common) (deviceIDCSR_s_org) (deviceIDCSR_s_country)
+                        (aliasKeyCrt_version)
+                        (aliasKeyCrt_serialNumber)
+                        (aliasKeyCrt_i_common) (aliasKeyCrt_i_org) (aliasKeyCrt_i_country)
+                        (aliasKeyCrt_notBefore) (aliasKeyCrt_notAfter)
+                        (aliasKeyCrt_s_common) (aliasKeyCrt_s_org) (aliasKeyCrt_s_country)
+                        (aliasKeyCrt_ku)
+                        (riot_version)
+                        (aliasKey_pub)
+                        (aliasKey_priv)
                         (deviceIDCSR_len) (deviceIDCSR_buf)
                         (aliasKeyCRT_len) (aliasKeyCRT_buf))
 = HST.push_frame ();
@@ -483,19 +389,20 @@ let riot
 
 (* Create DeviceIDCRI *)
    let deviceIDCRI_len: asn1_TLV_int32_of_type SEQUENCE = len_of_deviceIDCRI
-                                                            deviceIDCSR_ingredients.deviceIDCSR_version
-                                                            deviceIDCSR_ingredients.deviceIDCSR_s_common
-                                                            deviceIDCSR_ingredients.deviceIDCSR_s_org
-                                                            deviceIDCSR_ingredients.deviceIDCSR_s_country in
+                                                            deviceIDCSR_version
+                                                            deviceIDCSR_s_common
+                                                            deviceIDCSR_s_org
+                                                            deviceIDCSR_s_country
+                                                            deviceIDCSR_ku in
    let deviceIDCRI_buf: B.lbuffer byte_pub (v deviceIDCRI_len) = B.alloca 0x00uy deviceIDCRI_len in
 
    printf "Creating DeviceID Certificate Signing Request Information\n" done;
    create_deviceIDCRI
-    (* version   *) deviceIDCSR_ingredients.deviceIDCSR_version
-                    deviceIDCSR_ingredients.deviceIDCSR_s_common
-                    deviceIDCSR_ingredients.deviceIDCSR_s_org
-                    deviceIDCSR_ingredients.deviceIDCSR_s_country
-    (* key usage *) deviceIDCSR_ingredients.deviceIDCSR_ku
+    (* version   *) deviceIDCSR_version
+                    deviceIDCSR_s_common
+                    deviceIDCSR_s_org
+                    deviceIDCSR_s_country
+    (* key usage *) deviceIDCSR_ku
     (* DeviceID  *) deviceID_pub
     (*DeviceIDCRI*) deviceIDCRI_len
                     deviceIDCRI_buf;
@@ -510,32 +417,24 @@ let riot
                     deviceIDCSR_buf;
 (* Create AliasKeyTBS *)
   let aliasKeyTBS_len: asn1_TLV_int32_of_type SEQUENCE = len_of_aliasKeyTBS
-                                                           aliasKeyCRT_ingredients.aliasKeyCrt_serialNumber
-                                                           aliasKeyCRT_ingredients.aliasKeyCrt_i_common
-                                                           aliasKeyCRT_ingredients.aliasKeyCrt_i_org
-                                                           aliasKeyCRT_ingredients.aliasKeyCrt_i_country
-                                                           aliasKeyCRT_ingredients.aliasKeyCrt_s_common
-                                                           aliasKeyCRT_ingredients.aliasKeyCrt_s_org
-                                                           aliasKeyCRT_ingredients.aliasKeyCrt_s_country
-                                                           aliasKeyCRT_ingredients.aliasKeyCrt_riot_version in
+                                                           aliasKeyCrt_serialNumber
+                                                           aliasKeyCrt_i_common aliasKeyCrt_i_org aliasKeyCrt_i_country
+                                                           aliasKeyCrt_s_common aliasKeyCrt_s_org aliasKeyCrt_s_country
+                                                           aliasKeyCrt_ku
+                                                           riot_version in
   let aliasKeyTBS_buf: B.lbuffer byte_pub (v aliasKeyTBS_len) = B.alloca 0x00uy aliasKeyTBS_len in
 
   printf "Creating AliasKey Certificate TBS\n" done;
   create_aliasKeyTBS
-    (aliasKeyCRT_ingredients.aliasKeyCrt_version)
-    (aliasKeyCRT_ingredients.aliasKeyCrt_serialNumber)
-    (aliasKeyCRT_ingredients.aliasKeyCrt_i_common)
-    (aliasKeyCRT_ingredients.aliasKeyCrt_i_org)
-    (aliasKeyCRT_ingredients.aliasKeyCrt_i_country)
-    (aliasKeyCRT_ingredients.aliasKeyCrt_notBefore)
-    (aliasKeyCRT_ingredients.aliasKeyCrt_notAfter)
-    (aliasKeyCRT_ingredients.aliasKeyCrt_s_common)
-    (aliasKeyCRT_ingredients.aliasKeyCrt_s_org)
-    (aliasKeyCRT_ingredients.aliasKeyCrt_s_country)
+    (aliasKeyCrt_version)
+    (aliasKeyCrt_serialNumber)
+    (aliasKeyCrt_i_common) (aliasKeyCrt_i_org) (aliasKeyCrt_i_country)
+    (aliasKeyCrt_notBefore) (aliasKeyCrt_notAfter)
+    (aliasKeyCrt_s_common) (aliasKeyCrt_s_org) (aliasKeyCrt_s_country)
     (fwid)
-    (aliasKeyCRT_ingredients.aliasKeyCrt_ku)
+    (aliasKeyCrt_ku)
     (aliasKeyCrt_keyID)
-    (aliasKeyCRT_ingredients.aliasKeyCrt_riot_version)
+    (riot_version)
     (* DeviceID  *) deviceID_pub
     (* AliasKey  *) aliasKey_pub
     (*AliasKeyTBS*) aliasKeyTBS_len
