src/riot/RIoT.X509.AliasKeyTBS.Extensions.fsti
@@ -90,21 +90,21 @@ val lemma_serialize_aliasKeyTBS_extensions_payload_unfold
   (serialize_riot_extension `serialize` x.aliasKeyTBS_extensions_riot)
 )
 
-let valid_aliasKeyTBS_extensions_payload_ingredients
-  (version: datatype_of_asn1_type INTEGER)
-: Type0
-= v (len_of_x509_key_usage ()) +
-  length_of_aliasKeyTBS_extensions_extendedKeyUsage () +
-  length_of_aliasKeyTBS_extensions_basicConstraints () +
-  length_of_aliasKeyTBS_extensions_authKeyID () +
-  length_of_riot_extension version
-  <= asn1_value_length_max_of_type SEQUENCE
+// let valid_aliasKeyTBS_extensions_payload_ingredients
+//   (version: datatype_of_asn1_type INTEGER)
+// : Type0
+// = v (len_of_x509_key_usage ()) +
+//   length_of_aliasKeyTBS_extensions_extendedKeyUsage () +
+//   length_of_aliasKeyTBS_extensions_basicConstraints () +
+//   length_of_aliasKeyTBS_extensions_authKeyID () +
+//   length_of_riot_extension version
+//   <= asn1_value_length_max_of_type SEQUENCE
 
-val lemma_aliasKeyTBS_extensions_payload_ingredients_valid
-  (version: datatype_of_asn1_type INTEGER)
-: Lemma (
-  valid_aliasKeyTBS_extensions_payload_ingredients version
-)
+// val lemma_aliasKeyTBS_extensions_payload_ingredients_valid
+//   (version: datatype_of_asn1_type INTEGER)
+// : Lemma (
+//   valid_aliasKeyTBS_extensions_payload_ingredients version
+// )
 
 noextract inline_for_extraction unfold
 [@@ "opaque_to_smt"]
@@ -119,26 +119,24 @@ let len_of_aliasKeyTBS_extensions_payload_max ()
 let len_of_aliasKeyTBS_extensions_payload
   (version: datatype_of_asn1_type INTEGER)
 : Tot (asn1_value_int32_of_type SEQUENCE)
-= lemma_aliasKeyTBS_extensions_payload_ingredients_valid version;
+= //lemma_aliasKeyTBS_extensions_payload_ingredients_valid version;
   len_of_x509_key_usage () +
   len_of_aliasKeyTBS_extensions_extendedKeyUsage () +
   len_of_aliasKeyTBS_extensions_basicConstraints () +
   len_of_aliasKeyTBS_extensions_authKeyID () +
   len_of_riot_extension version
 
+let lemma_length_of_aliasKeyTBS_extensions_payload_size_max
+  (version: datatype_of_asn1_type INTEGER)
+: Lemma (
+  v (len_of_aliasKeyTBS_extensions_payload version)
+  <= v (len_of_aliasKeyTBS_extensions_payload_max ())
+)
+= ()
+
 val lemma_serialize_aliasKeyTBS_extensions_payload_size
   (x: aliasKeyTBS_extensions_payload_t)
 : Lemma (
-  lemma_serialize_aliasKeyTBS_extensions_payload_unfold x;
-    lemma_serialize_x509_key_usage_size_exact x.aliasKeyTBS_extensions_key_usage;
-    lemma_x509_keyPurposeIDs_unique aliasKeyCrt_extendedKeyUsage_oids;
-    lemma_serialize_aliasKeyTBS_extensions_extendedKeyUsage_size_exact
-                                              x.aliasKeyTBS_extensions_extendedKeyUsage;
-    lemma_serialize_aliasKeyTBS_extensions_basicConstraints_size_exact
-                                              x.aliasKeyTBS_extensions_basicConstraints;
-    lemma_serialize_aliasKeyTBS_extensions_authKeyID_size_exact
-                                              x.aliasKeyTBS_extensions_authKeyID;
-    lemma_serialize_riot_extension_size_exact x.aliasKeyTBS_extensions_riot;
   (* unfold *)
   length_of_opaque_serialization (serialize_aliasKeyTBS_extensions_payload)      x ==
   length_of_opaque_serialization (serialize_x509_key_usage)              x.aliasKeyTBS_extensions_key_usage +
@@ -156,6 +154,17 @@ val lemma_serialize_aliasKeyTBS_extensions_payload_size
   length_of_opaque_serialization (serialize_aliasKeyTBS_extensions_payload)      x
   <= v (len_of_aliasKeyTBS_extensions_payload_max ())
 )
+// = lemma_length_of_aliasKeyTBS_extensions_payload_size_max x.aliasKeyTBS_extensions_riot.x509_extValue_riot.riot_version;
+//   lemma_serialize_aliasKeyTBS_extensions_payload_unfold x;
+//     lemma_serialize_x509_key_usage_size_exact x.aliasKeyTBS_extensions_key_usage;
+//     lemma_x509_keyPurposeIDs_unique aliasKeyCrt_extendedKeyUsage_oids;
+//     lemma_serialize_aliasKeyTBS_extensions_extendedKeyUsage_size_exact
+//                                               x.aliasKeyTBS_extensions_extendedKeyUsage;
+//     lemma_serialize_aliasKeyTBS_extensions_basicConstraints_size_exact
+//                                               x.aliasKeyTBS_extensions_basicConstraints;
+//     lemma_serialize_aliasKeyTBS_extensions_authKeyID_size_exact
+//                                               x.aliasKeyTBS_extensions_authKeyID;
+//     lemma_serialize_riot_extension_size_exact x.aliasKeyTBS_extensions_riot
 
 (*
  * SEQUENCE serializer
@@ -190,30 +199,30 @@ val lemma_serialize_aliasKeyTBS_extensions_size
   (x: aliasKeyTBS_extensions_t)
 : Lemma ( predicate_serialize_asn1_sequence_TLV_size serialize_aliasKeyTBS_extensions_payload x )
 
-let valid_aliasKeyTBS_extensions_ingredients
-  (version: datatype_of_asn1_type INTEGER)
-: Type0
-= valid_aliasKeyTBS_extensions_payload_ingredients version /\
-  v (len_of_aliasKeyTBS_extensions_payload version)
-  <= asn1_value_length_max_of_type SEQUENCE
+// let valid_aliasKeyTBS_extensions_ingredients
+//   (version: datatype_of_asn1_type INTEGER)
+// : Type0
+// = valid_aliasKeyTBS_extensions_payload_ingredients version /\
+//   v (len_of_aliasKeyTBS_extensions_payload version)
+//   <= asn1_value_length_max_of_type SEQUENCE
 
-val lemma_aliasKeyTBS_extensions_ingredients_valid
-  (version: datatype_of_asn1_type INTEGER)
-: Lemma (
-  valid_aliasKeyTBS_extensions_ingredients version
-)
+// val lemma_aliasKeyTBS_extensions_ingredients_valid
+//   (version: datatype_of_asn1_type INTEGER)
+// : Lemma (
+//   valid_aliasKeyTBS_extensions_ingredients version
+// )
 
-let valid_aliasKeyTBS_extensions
-  (x: aliasKeyTBS_extensions_t)
-: Type0
-= valid_aliasKeyTBS_extensions_ingredients
-          (x.aliasKeyTBS_extensions_riot.x509_extValue_riot.riot_version)
+// let valid_aliasKeyTBS_extensions
+//   (x: aliasKeyTBS_extensions_t)
+// : Type0
+// = valid_aliasKeyTBS_extensions_ingredients
+//           (x.aliasKeyTBS_extensions_riot.x509_extValue_riot.riot_version)
 
-val lemma_aliasKeyTBS_extensions_valid
-  (x: aliasKeyTBS_extensions_t)
-: Lemma (
-  valid_aliasKeyTBS_extensions x
-)
+// val lemma_aliasKeyTBS_extensions_valid
+//   (x: aliasKeyTBS_extensions_t)
+// : Lemma (
+//   valid_aliasKeyTBS_extensions x
+// )
 
 noextract inline_for_extraction unfold
 [@@ "opaque_to_smt"]
@@ -225,14 +234,14 @@ let len_of_aliasKeyTBS_extensions_max ()
 let len_of_aliasKeyTBS_extensions
   (version: datatype_of_asn1_type INTEGER)
 : Tot (asn1_TLV_int32_of_type SEQUENCE)
-= lemma_aliasKeyTBS_extensions_ingredients_valid version;
+= //lemma_aliasKeyTBS_extensions_ingredients_valid version;
   len_of_TLV SEQUENCE
     (len_of_aliasKeyTBS_extensions_payload version)
 
 val lemma_serialize_aliasKeyTBS_extensions_size_exact
   (x: aliasKeyTBS_extensions_t)
 : Lemma (
-  Classical.forall_intro lemma_aliasKeyTBS_extensions_ingredients_valid;
+  // Classical.forall_intro lemma_aliasKeyTBS_extensions_ingredients_valid;
   (* exact size *)
   length_of_opaque_serialization (serialize_aliasKeyTBS_extensions) x
   == v (len_of_aliasKeyTBS_extensions
@@ -261,7 +270,7 @@ let x509_get_aliasKeyTBS_extensions
   (deviceIDPub: B32.lbytes32 32ul)
 : Tot (aliasKeyTBS_extensions_t)
 =
-  (* Prf*) Classical.forall_intro lemma_aliasKeyTBS_extensions_ingredients_valid;
+  // (* Prf*) Classical.forall_intro lemma_aliasKeyTBS_extensions_ingredients_valid;
 
   let key_usage = x509_get_key_usage ku in
   (* Prf *) lemma_serialize_x509_key_usage_size_exact key_usage;
