src/riot/RIoT.X509.Base.fst
@@ -1,11 +1,10 @@
 module RIoT.X509.Base
 open ASN1.Spec
 open RIoT.Base
-open X509
+open X509.Base
+open X509.ExtFields.KeyUsage
 
 module B32 = FStar.Bytes
-
-#set-options "--z3rlimit 32 --fuel 0 --ifuel 0"
 
 let aliasKeyCrt_key_usage: key_usage_payload_t
 = normalize_term (x509_KU_KEY_CERT_SIGN
@@ -14,42 +13,21 @@ let aliasKeyCrt_key_usage: key_usage_payload_t
    * [reference implementation](https://github.com/microsoft/RIoT/blob/master/Reference/RIoT/RIoTCrypt/include/x509bldr.h#L22),
    * Only the KeyCertSign bit is set.
    *)
-  `op_ku_with` x509_KU_DIGITAL_SIGNATURE
-  `op_ku_with` x509_KU_CRL_SIGN)
+  // `op_ku_with` x509_KU_DIGITAL_SIGNATURE
+  // `op_ku_with` x509_KU_CRL_SIGN
+  )
 
-let sha1_digest_to_octet_string_spec
-  (s: lbytes_pub 20)
-: GTot (x: datatype_of_asn1_type OCTET_STRING
-           { dfst x == 20ul /\
-             B32.reveal (dsnd x) == s })
-= assert_norm (Seq.length s < pow2 32);
-  let s32: B32.lbytes 20 = B32.hide s in
-  B32.reveal_hide s;
-  assert (B32.reveal s32 == s);
-  (|20ul, s32|)
+// let sha1_digest_to_octet_string_spec
+//   (s: lbytes_pub 20)
+// : GTot (x: datatype_of_asn1_type OCTET_STRING
+//            { dfst x == 20ul /\
+//              B32.reveal (dsnd x) == s })
+// = assert_norm (Seq.length s < pow2 32);
+//   let s32: B32.lbytes 20 = B32.hide s in
+//   B32.reveal_hide s;
+//   assert (B32.reveal s32 == s);
+//   (|20ul, s32|)
 
-type deviceIDCSR_ingredients_t = {
-  deviceIDCSR_ku: key_usage_payload_t;
-  deviceIDCSR_version: datatype_of_asn1_type INTEGER;
-  deviceIDCSR_s_common:  x509_RDN_x520_attribute_string_t COMMON_NAME  IA5_STRING;
-  deviceIDCSR_s_org:     x509_RDN_x520_attribute_string_t ORGANIZATION IA5_STRING;
-  deviceIDCSR_s_country: x509_RDN_x520_attribute_string_t COUNTRY      PRINTABLE_STRING
-}
-
-type aliasKeyCRT_ingredients_t = {
-  aliasKeyCrt_version: x509_version_t;
-  aliasKeyCrt_serialNumber: x509_serialNumber_t;
-  aliasKeyCrt_i_common:  x509_RDN_x520_attribute_string_t COMMON_NAME  IA5_STRING;
-  aliasKeyCrt_i_org:     x509_RDN_x520_attribute_string_t ORGANIZATION IA5_STRING;
-  aliasKeyCrt_i_country: x509_RDN_x520_attribute_string_t COUNTRY      PRINTABLE_STRING;
-  aliasKeyCrt_notBefore: datatype_of_asn1_type Generalized_Time;
-  aliasKeyCrt_notAfter : datatype_of_asn1_type Generalized_Time;
-  aliasKeyCrt_s_common:  x509_RDN_x520_attribute_string_t COMMON_NAME  IA5_STRING;
-  aliasKeyCrt_s_org:     x509_RDN_x520_attribute_string_t ORGANIZATION IA5_STRING;
-  aliasKeyCrt_s_country: x509_RDN_x520_attribute_string_t COUNTRY      PRINTABLE_STRING;
-  aliasKeyCrt_ku: key_usage_payload_t;
-  aliasKeyCrt_riot_version: datatype_of_asn1_type INTEGER;
-}
 
 // inline_for_extraction
 // let alg_DeviceID = AlgID_Ed25519
